new commit

Automata/Common.lean
@@ -2,6 +2,7 @@ import Mathlib.Tactic
 import Mathlib.Data.List.Basic
 import Automata.DFA
 import Automata.NFA
+import Automata.Input
 import Mathlib.Data.Nat.Digits
 
 def thueMorse : DFAO (Fin 2) (Fin 2) (Fin 2) := {
@@ -10,34 +11,10 @@ def thueMorse : DFAO (Fin 2) (Fin 2) (Fin 2) := {
   output := fun x => x
 }
 
-#eval thueMorse.eval [0]
-#eval thueMorse.eval [1]
-#eval thueMorse.eval [1, 0]
-#eval thueMorse.eval [1, 1]
-#eval thueMorse.eval [1, 0, 0]
-#eval thueMorse.eval [1, 0, 1]
-#eval thueMorse.eval [1, 1, 0]
-#eval thueMorse.eval [1, 1, 1]
 
 def thueMorse0 : DFA (Fin 2) (Fin 2) := thueMorse.toDFA 0
-#eval thueMorse0.eval [0]
-#eval thueMorse0.eval [1]
-#eval thueMorse0.eval [1, 0]
-#eval thueMorse0.eval [1, 1]
-#eval thueMorse0.eval [1, 0, 0]
-#eval thueMorse0.eval [1, 0, 1]
-#eval thueMorse0.eval [1, 1, 0]
-#eval thueMorse0.eval [1, 1, 1]
 
 def thueMorse1 : DFA (Fin 2) (Fin 2) := thueMorse.toDFA 1
-#eval thueMorse1.eval [0]
-#eval thueMorse1.eval [1]
-#eval thueMorse1.eval [1, 0]
-#eval thueMorse1.eval [1, 1]
-#eval thueMorse1.eval [1, 0, 0]
-#eval thueMorse1.eval [1, 0, 1]
-#eval thueMorse1.eval [1, 1, 0]
-#eval thueMorse1.eval [1, 1, 1]
 
 def trueDFA: DFA (Fin 0) (Fin 1) := {
   transition := fun _ s => s
@@ -51,10 +28,6 @@ def falseDFA: DFA (Fin 0) (Fin 1) := {
   output := fun _ => false
 }
 
-#eval trueDFA.eval []
-#eval falseDFA.eval []
-
-
 def eqBase (k: ℕ) : DFA (Fin 2 → Fin k) (Fin 2) := {
   transition := fun f s => match s with
     | 0 => if (f 0).val == f 1 then 0 else 1
@@ -62,6 +35,9 @@ def eqBase (k: ℕ) : DFA (Fin 2 → Fin k) (Fin 2) := {
   start := 0
   output := fun x => x == 0
 }
+
+--Exists x, x = 0?
+#eval (project (eqBase 2) (by norm_num) ⟨0, by norm_num⟩).eval [fun _ => 0]
 
 def eqBase' (k: ℕ) (a b n : ℕ) (ha: a < n) (hb: b < n): DFA (Fin n → Fin k) (Fin 2) := {
   transition := fun f s => match s with
@@ -75,7 +51,6 @@ def eqBase' (k: ℕ) (a b n : ℕ) (ha: a < n) (hb: b < n): DFA (Fin n → Fin k
 #eval (eqBase 2).eval [fun x => x, fun x => x]
 #eval (eqBase' 2 0 1 2 (by norm_num) (by norm_num)).eval [fun _ => 0, fun _ => 1]
 #eval (eqBase' 2 0 1 2 (by norm_num) (by norm_num)).eval [fun x => x, fun x => x]
-
 
 def addBase (k: ℕ) : DFA (Fin 3 → Fin k) (Fin 3) := {
   transition := fun f s => match s with
@@ -99,73 +74,43 @@ def ltBase (k: ℕ)  : DFA (Fin 2 → Fin k) (Fin 3) := {
   output := fun x => x == 1
 }
 
-def digits' (b: ℕ) (n: ℕ) (h: b > 1) : List (Fin b) :=
-  (Nat.digits b n).attach.map (fun x => ⟨x.1, Nat.digits_lt_base h x.2⟩)
+-- Exists x, x < 0?
+#eval (project (ltBase 2) (by norm_num) ⟨0, by norm_num⟩).eval [fun _ => 0]
 
-#eval digits' 2 12 (by norm_num)
-
-def toBase (b : ℕ) (n : ℕ): List ℕ :=
-  (Nat.digits b n).reverse
-
-def ofBase (b : ℕ) (l : List ℕ) : ℕ :=
-  l.foldl (fun x y => x * b + y) 0
-
-theorem ofBase_toBase (b: ℕ) (n: ℕ) : ofBase b (toBase b n) = n := by
-  simp only [toBase, ofBase, List.foldl_reverse, add_comm, mul_comm]
-  have h: Nat.ofDigits b (b.digits n) = n := Nat.ofDigits_digits b n
-  nth_rewrite 2 [← h]
-  rw [Nat.ofDigits_eq_foldr]
-  rfl
+--Exists x, x + 1 = 0? Wrong Answer!
+#eval (project (addBase 2) (by norm_num) ⟨0, by norm_num⟩).evalFrom [fun x => if x == 0 then 1 else 0] [0]
 
 
-def addLeadingZeros (n: ℕ) (l: List ℕ): List ℕ :=
-  (List.replicate n 0) ++ l
 
-theorem addLeadingZerosLength (n: ℕ) (l: List ℕ) :
-  (addLeadingZeros n l).length = n + l.length :=
-  by simp only [addLeadingZeros, List.length_append, List.length_replicate]
-
-theorem ofBase_addLeadingZeros (b: ℕ)(n: ℕ) (l: List ℕ) :
-  ofBase b (addLeadingZeros n l) = ofBase b l := by
-  simp only [ofBase, addLeadingZeros]
-  induction n
-  case zero => simp
-  case succ n ih =>
-    simp [addLeadingZeros, List.replicate, List.foldl, ih]
-
-def mapToBase (b: ℕ) (l: List ℕ) : List (List ℕ) :=
-  l.map (toBase b)
-
-def maxLen : (l: List (List α)) → ℕ
-  | [] => 0
-  | x :: xs => max x.length (maxLen xs)
-
-theorem cons_lt_maxLen (l: List α) (ls: List (List α)) :
-  l.length ≤ maxLen (l :: ls) := by
-  induction ls generalizing l with
-  | nil => simp[maxLen]
-  | cons head tail _ =>
-    simp [maxLen]
-
-
-theorem len_lt_maxLen (l: List α) (ls: List (List α)) :
-  l ∈ ls → l.length ≤ maxLen ls := by
+theorem eqBase_if_equal_aux (b : ℕ) (m n : ℕ) (hb: b > 1):
+  m = n → (eqBase b).evalFrom (inputToBase b hb [m, n]) 0 := by
   intro h
-  induction ls generalizing l with
-  | nil => simp only [List.not_mem_nil] at h
-  | cons head tail ih =>
-    have h1: l = head ∨ l ∈ tail := List.eq_or_mem_of_mem_cons h
-    rcases h1 with (rfl | h1)
-    . apply cons_lt_maxLen
-    . simp[maxLen]
-      right
-      exact ih l h1
-
-def toBaseZip (b : ℕ) (hb: b > 1) (l: List ℕ) : (List (Fin l.length → Fin b)) :=
+  rw[h]
+  generalize hl: (inputToBase b hb [n, n]).length = l
+  induction l with
+  | zero =>
+    simp only [List.length_eq_zero] at hl
+    rw[hl]
+    simp[eqBase, DFAO.evalFrom]
+  | succ l ih =>
 
 
+  sorry
 
 
+
+theorem eqBase_if_equal (b : ℕ) (m n : ℕ) (hb: b > 1):
+  m = n → (eqBase b).eval (inputToBase b hb [m, n]) := by
+  rw[DFAO.eval]
+  intro h
+  rw[h]
+  generalize hl: (inputToBase b hb [n, n]).length = l
+  induction l with
+  | zero =>
+    simp only [List.length_eq_zero] at hl
+    rw[hl]
+    simp[eqBase, DFAO.evalFrom]
+  | succ l ih =>
 
 
   sorry
