Automata/Input.lean
@@ -1,0 +1,282 @@
+import Mathlib.Tactic
+import Mathlib.Data.List.Basic
+import Mathlib.Data.Nat.Digits
+
+/-
+Idea: Given a list of natural numbers 'l',
+
+Step 1: Convert each number to base b, get 'ls' : List (List ℕ)
+
+Step 2: Stretch each list to uniform length by adding leading zeros, get 'lss' : List (List ℕ)
+
+Step 2.5? : Convert 'lss' to List (List (Fin b)) using 'toBase_lt_base'
+
+Step 3: Zip the lists together to get the input to automatas: List (Fin (l.length) → Fin b)
+-/
+
+--def digits' (b: ℕ) (n: ℕ) (h: b > 1) : List (Fin b) :=
+--  (Nat.digits b n).attach.map (fun x => ⟨x.1, Nat.digits_lt_base h x.2⟩)
+
+def toBase (b : ℕ) (n : ℕ): List ℕ :=
+  (Nat.digits b n).reverse
+
+theorem toBase_lt_base (b: ℕ) (n: ℕ) (hb: b > 1) :
+  x ∈ (toBase b n) → x < b := by
+  intro h
+  simp only [toBase] at h
+  have h1: x ∈ Nat.digits b n := List.mem_reverse.mp h
+  apply Nat.digits_lt_base
+  exact hb
+  exact h1
+
+def ofBase (b : ℕ) (l : List ℕ) : ℕ :=
+  l.foldl (fun x y => x * b + y) 0
+
+theorem ofBase_toBase (b: ℕ) (n: ℕ) : ofBase b (toBase b n) = n := by
+  simp only [toBase, ofBase, List.foldl_reverse, add_comm, mul_comm]
+  have h: Nat.ofDigits b (b.digits n) = n := Nat.ofDigits_digits b n
+  nth_rewrite 2 [← h]
+  rw [Nat.ofDigits_eq_foldr]
+  rfl
+
+def addLeadingZeros (n: ℕ) (l: List ℕ): List ℕ :=
+  (List.replicate n 0) ++ l
+
+theorem addLeadingZeros_elem (n: ℕ) (l: List ℕ) :
+  x ∈ (addLeadingZeros n l) → x = 0 ∨ x ∈ l := by
+  intro h
+  simp only [addLeadingZeros, List.mem_append, List.replicate] at h
+  rcases h with (h | h)
+  . left
+    have : x ∈ [0] := List.replicate_subset_singleton n 0 h
+    exact Finset.mem_zero.mp this
+  . right
+    exact h
+
+#check List.replicate_subset_singleton 3 0
+
+theorem addLeadingZerosLength (n: ℕ) (l: List ℕ) :
+  (addLeadingZeros n l).length = n + l.length :=
+  by simp only [addLeadingZeros, List.length_append, List.length_replicate]
+
+theorem ofBase_addLeadingZeros (b: ℕ)(n: ℕ) (l: List ℕ) :
+  ofBase b (addLeadingZeros n l) = ofBase b l := by
+  simp only [ofBase, addLeadingZeros]
+  induction n
+  case zero => simp
+  case succ n ih =>
+    simp [addLeadingZeros, List.replicate, List.foldl, ih]
+
+def maxLen : (l: List (List α)) → ℕ
+  | [] => 0
+  | x :: xs => max x.length (maxLen xs)
+
+theorem cons_lt_maxLen (l: List α) (ls: List (List α)) :
+  l.length ≤ maxLen (l :: ls) := by
+  induction ls generalizing l with
+  | nil => simp[maxLen]
+  | cons head tail _ =>
+    simp [maxLen]
+
+theorem len_lt_maxLen (l: List α) (ls: List (List α)) :
+  l ∈ ls → l.length ≤ maxLen ls := by
+  intro h
+  induction ls generalizing l with
+  | nil => simp only [List.not_mem_nil] at h
+  | cons head tail ih =>
+    have h1: l = head ∨ l ∈ tail := List.eq_or_mem_of_mem_cons h
+    rcases h1 with (rfl | h1)
+    . apply cons_lt_maxLen
+    . simp[maxLen]
+      right
+      exact ih l h1
+
+def mapToBase (b: ℕ) (l: List ℕ) : List (List ℕ) :=
+  l.map (toBase b)
+
+theorem mapToBase_lt_base (b: ℕ) (l: List ℕ) (hb: b > 1) :
+  ∀ x ∈ (mapToBase b l), ∀ y ∈ x, y < b  := by
+  intro x hx y hy
+  simp only [mapToBase, List.mem_map] at hx
+  rcases hx with ⟨z, _, rfl⟩
+  apply toBase_lt_base
+  exact hb
+  exact hy
+
+theorem mapToBase_length (b: ℕ) (l: List ℕ) : (mapToBase b l).length = l.length := by
+  simp only [mapToBase, List.length_map]
+
+def stretchLen (ls: List (List ℕ)) : List (List ℕ) :=
+  ls.map (fun l => addLeadingZeros (maxLen ls - l.length) l)
+
+theorem stretchLen_length (ls: List (List ℕ)) : (stretchLen ls).length = ls.length := by
+  simp only [stretchLen, List.length_map]
+
+theorem stretchLen_uniform (ls: List (List ℕ)) :
+  l ∈ stretchLen ls →  l.length = maxLen ls:= by
+  intro h
+  simp only [stretchLen, List.mem_map] at h
+  rcases h with ⟨x, hx, rfl⟩
+  simp only [addLeadingZerosLength]
+  have: x.length ≤ maxLen ls := len_lt_maxLen x ls hx
+  omega
+
+theorem stretchLen_of_mapToBase_lt_base (b: ℕ) (l: List ℕ) (hb: b > 1) :
+  ∀ x ∈ (stretchLen (mapToBase b l)), ∀ y ∈ x, y < b := by
+  intro x hx y hy
+  simp only [stretchLen, List.mem_map] at hx
+  rcases hx with ⟨z, left, rfl⟩
+  have h := addLeadingZeros_elem (maxLen (mapToBase b l) - z.length) z hy
+  rcases h with (rfl | h)
+  . omega
+  apply mapToBase_lt_base
+  . exact hb
+  . simp only [addLeadingZeros, List.replicate] at hy
+    exact left
+  . exact h
+
+theorem tailLen (l: List α) : l.tail.length = l.length - 1 := by
+  rcases l
+  . simp
+  . simp
+
+def zipToAlphabetFin (n : ℕ) (l : ℕ) (lss: List (List ℕ))
+(hlb: ∀ x ∈ lss, ∀ y ∈ x, y < b) (hlss: lss.length = l)
+(hls : ∀ ls ∈ lss, ls.length = n) : List (Fin l → Fin b) :=
+  match n with
+  | 0 => []
+  | m+1 =>
+     (fun i =>
+       have : 0 < lss[i].length := by
+         rw[hls]
+         omega
+         refine List.mem_iff_get.mpr ?_
+         subst hlss
+         use i
+         rfl
+
+       ⟨lss[i][0], (by
+          apply hlb lss[i]
+          . apply List.mem_iff_getElem.mpr
+            simp only [Fin.getElem_fin, hlss]
+            use i
+            use i.isLt
+          . apply List.mem_iff_getElem.mpr
+            use 0
+            use this)⟩
+        ) :: (zipToAlphabetFin m l (lss.map (fun ls => ls.tail))
+        (by
+          intro x hx
+          simp only [List.mem_map] at hx
+          rcases hx with ⟨s, hs, rfl⟩
+          intro y hy
+          specialize hlb s hs
+          apply hlb
+          exact List.mem_of_mem_tail hy
+        )
+        (by simp only [List.length_map, hlss]) (fun
+          | .nil => by
+            simp only [List.mem_map, List.length_nil, forall_exists_index, and_imp]
+            intro x hx
+            specialize hls x hx
+            rcases x
+            . simp only [List.length_nil, self_eq_add_left, AddLeftCancelMonoid.add_eq_zero,
+              one_ne_zero, and_false] at hls
+            . simp only [List.length_cons, add_left_inj] at hls
+              simp only [List.tail_cons]
+              intro h
+              simp only [h, List.length_nil] at hls
+              assumption
+          | .cons head tail => by
+            simp only [List.mem_map, List.length_cons, forall_exists_index, and_imp]
+            intro x hx h
+            specialize hls x hx
+            have : x.tail.length = m := by
+              have: x.length - 1 = m := by
+                omega
+              rw[← this]
+              apply tailLen x
+            rw[← this, h]
+            have hxtail := tailLen x.tail
+            rw[h, List.tail] at hxtail
+            have: (head :: tail).length > 0 := by simp
+            omega
+            ))
+
+theorem zipToAlphabetFin_length (n : ℕ) (l : ℕ) (lss: List (List ℕ))
+(hlb: ∀ x ∈ lss, ∀ y ∈ x, y < b) (hlss: lss.length = l)
+(hls : ∀ ls ∈ lss, ls.length = n) :
+  (zipToAlphabetFin n l lss hlb hlss hls).length = n := by
+  induction n generalizing l lss
+  case zero =>
+    simp only [List.length_eq_zero, zipToAlphabetFin]
+  case succ n ih =>
+    simp only [zipToAlphabetFin, add_left_inj, List.length_cons]
+    apply ih
+
+def inputToBase (b : ℕ) (hb: b > 1) (l: List ℕ) : List (Fin l.length → Fin b) :=
+  let ls := mapToBase b l
+  let n := maxLen ls
+  let lss := stretchLen (ls)
+  zipToAlphabetFin n l.length lss (by
+    apply stretchLen_of_mapToBase_lt_base
+    exact hb
+  ) (by simp only [mapToBase_length b l, stretchLen_length ls]) (by
+    intro ls hls
+    apply stretchLen_uniform
+    assumption)
+
+
+/-
+def zipToAlphabet (n : ℕ) (l : ℕ) (lss: List (List ℕ)) (hlss: lss.length = l) (hls : ∀ ls ∈ lss, ls.length = n) : List (Fin l → ℕ) :=
+  match n with
+  | 0 => []
+  | m+1 =>
+     (fun i =>
+       have : 0 < lss[i].length := by
+         rw[hls]
+         omega
+         refine List.mem_iff_get.mpr ?_
+         subst hlss
+         use i
+         rfl
+
+       lss[i][0]) :: (zipToAlphabet m l (lss.map (fun ls => ls.tail))
+        (by simp only [List.length_map, hlss]) (fun
+          | .nil => by
+            simp only [List.mem_map, List.length_nil, forall_exists_index, and_imp]
+            intro x hx
+            specialize hls x hx
+            rcases x
+            . simp only [List.length_nil, self_eq_add_left, AddLeftCancelMonoid.add_eq_zero,
+              one_ne_zero, and_false] at hls
+            . simp only [List.length_cons, add_left_inj] at hls
+              simp only [List.tail_cons]
+              intro h
+              simp only [h, List.length_nil] at hls
+              assumption
+          | .cons head tail => by
+            simp only [List.mem_map, List.length_cons, forall_exists_index, and_imp]
+            intro x hx h
+            specialize hls x hx
+            have : x.tail.length = m := by
+              have: x.length - 1 = m := by
+                omega
+              rw[← this]
+              apply tailLen x
+            rw[← this, h]
+            have hxtail := tailLen x.tail
+            rw[h, List.tail] at hxtail
+            have: (head :: tail).length > 0 := by simp
+            omega
+            ))
+
+def toBaseZip (b : ℕ) (l: List ℕ) : (List (Fin l.length → ℕ)) :=
+  let ls := mapToBase b l
+  let n := maxLen ls
+  let lss := stretchLen (ls)
+  zipToAlphabet n l.length lss (by simp only [mapToBase_length b l, stretchLen_length ls]) (by
+    intro ls hls
+    apply stretchLen_uniform
+    assumption)
+-/
